Streamline 3SAT to IS reduction for paper

HOL_To_IMP/Refinements/HOL_To_IMP_THREE_SAT_To_IS.thy
@@ -7,179 +7,89 @@ theory HOL_To_IMP_THREE_SAT_To_IS
 begin
 
 context HOL_To_HOL_Nat
-begin
+begin       
 
-definition "map_acc_rpair y \<equiv> map_acc (rpair y)"
-lemmas map_acc_rpair_eq = map_acc_eq[of "rpair y" for y, folded map_acc_rpair_def]
-function_compile_nat map_acc_rpair_eq
+lemmas sat_is_un_1_list_fo0_eq = sat_is_un_1_list_fo0_def[unfolded case_prod_unfold]
+function_compile_nat sat_is_un_1_list_fo0_eq
 
-definition "case_prod_map_rpair \<equiv> \<lambda>(x, xs). map (rpair x) xs"
-lemmas case_prod_map_rpair_eq = case_prod_map_rpair_def[unfolded map_eq_map_acc_nil,
-    folded map_acc_rpair_def]
-function_compile_nat case_prod_map_rpair_eq
+definition "map_acc_sat_is_un_1_list_fo0 i_C l1 \<equiv> map_acc (sat_is_un_1_list_fo0 i_C l1)"
+lemmas map_acc_sat_is_un_1_list_fo0_eq =
+  map_acc_eq[of "sat_is_un_1_list_fo0 i_C l1" for i_C l1, folded map_acc_sat_is_un_1_list_fo0_def]  
+function_compile_nat map_acc_sat_is_un_1_list_fo0_eq
 
-definition "map_acc_case_prod_map_rpair \<equiv> map_acc case_prod_map_rpair"
-lemmas map_acc_case_prod_map_rpair_eq = map_acc_eq[of "case_prod_map_rpair",
-  folded map_acc_case_prod_map_rpair_def]
-function_compile_nat map_acc_case_prod_map_rpair_eq
+lemmas sat_is_un_1_list_fo1_eq =
+  sat_is_un_1_list_fo1_def[unfolded case_prod_unfold map_eq_map_acc_nil,
+    folded map_acc_sat_is_un_1_list_fo0_def]
+function_compile_nat sat_is_un_1_list_fo1_eq
 
-end
+definition "map_acc_sat_is_un_1_list_fo1 i_C \<equiv> map_acc (sat_is_un_1_list_fo1 i_C)"
+lemmas map_acc_sat_is_un_1_list_fo1_eq =
+  map_acc_eq[of "sat_is_un_1_list_fo1 i_C" for i_C, folded map_acc_sat_is_un_1_list_fo1_def]
+function_compile_nat map_acc_sat_is_un_1_list_fo1_eq
 
-context HOL_Nat_To_IMP
-begin
+lemmas sat_is_un_1_list_fo2_eq =
+  sat_is_un_1_list_fo2_def[unfolded case_prod_unfold map_eq_map_acc_nil,
+    folded map_acc_sat_is_un_1_list_fo1_def]
+function_compile_nat sat_is_un_1_list_fo2_eq
 
-lemmas map_acc_rpair_nat_eq = HTHN.map_acc_rpair_nat_eq_unfolded[unfolded case_list_nat_def]
-compile_nat map_acc_rpair_nat_eq
-HOL_To_IMP_correct HOL_To_HOL_Nat.map_acc_rpair_nat
-  apply (tactic \<open>HM.correct_if_IMP_tailcall_correct_tac HT.get_IMP_def @{context} 1\<close>)
-  by (induction "HTHN.rpair y :: 'b \<Rightarrow> _" _ _ arbitrary: s rule: HTHN.map_acc.induct)
-  (cook mode = run_finish)
+definition "map_acc_sat_is_un_1_list_fo2 \<equiv> map_acc (sat_is_un_1_list_fo2)"
+lemmas map_acc_sat_is_un_1_list_fo2_eq =
+  map_acc_eq[of "sat_is_un_1_list_fo2", folded map_acc_sat_is_un_1_list_fo2_def]
+function_compile_nat map_acc_sat_is_un_1_list_fo2_eq
 
-lemmas case_prod_map_rpair_nat_eq = HTHN.case_prod_map_rpair_nat_eq_unfolded[unfolded
-  case_prod_nat_def]
-compile_nat case_prod_map_rpair_nat_eq
-HOL_To_IMP_correct HOL_To_HOL_Nat.case_prod_map_rpair_nat by (cook mode = induction)
-
-lemmas map_acc_case_prod_map_rpair_nat_eq =
-  HTHN.map_acc_case_prod_map_rpair_nat_eq_unfolded[unfolded case_list_nat_def]
-compile_nat map_acc_case_prod_map_rpair_nat_eq
-HOL_To_IMP_correct HOL_To_HOL_Nat.map_acc_case_prod_map_rpair_nat
-  apply (tactic \<open>HM.correct_if_IMP_tailcall_correct_tac HT.get_IMP_def @{context} 1\<close>)
-  by (induction "HTHN.case_prod_map_rpair :: ('a \<times> 'b list) \<Rightarrow> _" _ _ arbitrary: s
-    rule: HTHN.map_acc.induct)
-  (cook mode = run_finish)
-
-end
-
-context HOL_To_HOL_Nat
-begin
-
-definition "map_acc_product \<equiv> map_acc (\<lambda>x. List.product x x)"
-lemmas map_acc_product_eq = map_acc_eq[of "\<lambda>x. List.product x x", folded map_acc_product_def]
-function_compile_nat map_acc_product_eq
+lemmas sat_is_un_1_list_fo_eq =
+  sat_is_un_1_list_fo_def[unfolded map_eq_map_acc_nil, folded map_acc_sat_is_un_1_list_fo2_def]
+function_compile_nat sat_is_un_1_list_fo_eq
 
 end
 
 context HOL_Nat_To_IMP
 begin
 
-lemmas map_acc_product_nat_eq = HTHN.map_acc_product_nat_eq_unfolded[unfolded case_list_nat_def]
-compile_nat map_acc_product_nat_eq
-HOL_To_IMP_correct HOL_To_HOL_Nat.map_acc_product_nat
+lemmas sat_is_un_1_list_fo0_nat_eq =
+  HTHN.sat_is_un_1_list_fo0_nat_eq_unfolded[unfolded case_prod_nat_def]
+compile_nat sat_is_un_1_list_fo0_nat_eq
+HOL_To_IMP_correct HOL_To_HOL_Nat.sat_is_un_1_list_fo0_nat
+  by cook
+
+lemmas map_acc_sat_is_un_1_list_fo0_nat_eq =
+  HTHN.map_acc_sat_is_un_1_list_fo0_nat_eq_unfolded[unfolded case_list_nat_def]
+compile_nat map_acc_sat_is_un_1_list_fo0_nat_eq
+HOL_To_IMP_correct HOL_To_HOL_Nat.map_acc_sat_is_un_1_list_fo0_nat
   apply (tactic \<open>HM.correct_if_IMP_tailcall_correct_tac HT.get_IMP_def @{context} 1\<close>)
-  by (induction "\<lambda>x :: 'a list. List.product x x" _ _ arbitrary: s rule: HTHN.map_acc.induct)
-  (cook mode = run_finish)
+  apply(induction "sat_is_un_1_list_fo0 y ya" _ _ arbitrary: s rule: HTHN.map_acc.induct)
+   apply(cook mode = run_finish)
+  done
 
-end
+compile_nat HTHN.sat_is_un_1_list_fo1_nat_eq_unfolded
+HOL_To_IMP_correct HOL_To_HOL_Nat.sat_is_un_1_list_fo1_nat
+  by cook
 
-context HOL_To_HOL_Nat
-begin
-definition "prod_fsts_neq \<equiv> \<lambda>((a, _), (b, _)). a \<noteq> b"
-function_compile_nat prod_fsts_neq_def
-
-definition "filter_acc_prod_fsts_neq \<equiv> filter_acc prod_fsts_neq"
-lemmas filter_prod_fsts_neq_acc_eq = filter_acc_eq[of prod_fsts_neq, folded
-  filter_acc_prod_fsts_neq_def]
-function_compile_nat filter_prod_fsts_neq_acc_eq
-
-definition "filter_prod_fsts_neq \<equiv> filter prod_fsts_neq"
-lemmas filter_prod_fsts_neq_eq = filter_prod_fsts_neq_def[unfolded filter_eq_filter_acc_nil,
-  folded filter_acc_prod_fsts_neq_def]
-function_compile_nat filter_prod_fsts_neq_eq
-
-definition "map_acc_filter_prod_fsts_neq \<equiv> map_acc filter_prod_fsts_neq"
-lemmas map_filter_prod_fsts_neq_acc_eq = map_acc_eq[of filter_prod_fsts_neq,
-  folded map_acc_filter_prod_fsts_neq_def]
-function_compile_nat map_filter_prod_fsts_neq_acc_eq
-
-end
-
-context HOL_Nat_To_IMP
-begin
-
-lemmas prod_fsts_neq_nat_eq = HTHN.prod_fsts_neq_nat_eq_unfolded[unfolded case_prod_nat_def]
-compile_nat prod_fsts_neq_nat_eq
-HOL_To_IMP_correct HOL_To_HOL_Nat.prod_fsts_neq_nat by cook
-
-lemmas filter_prod_fsts_neq_acc_nat_eq = HTHN.filter_acc_prod_fsts_neq_nat_eq_unfolded[unfolded
-  case_bool_nat_def case_list_nat_def]
-compile_nat filter_prod_fsts_neq_acc_nat_eq
-HOL_To_IMP_correct HOL_To_HOL_Nat.filter_acc_prod_fsts_neq_nat
+lemmas map_acc_sat_is_un_1_list_fo1_nat_eq =
+  HTHN.map_acc_sat_is_un_1_list_fo1_nat_eq_unfolded[unfolded case_list_nat_def]
+compile_nat map_acc_sat_is_un_1_list_fo1_nat_eq
+HOL_To_IMP_correct HOL_To_HOL_Nat.map_acc_sat_is_un_1_list_fo1_nat
   apply (tactic \<open>HM.correct_if_IMP_tailcall_correct_tac HT.get_IMP_def @{context} 1\<close>)
-  by (induction "HTHN.prod_fsts_neq :: ((('a \<times> 'b) \<times> ('a \<times> 'c)) \<Rightarrow> bool) " _ _ arbitrary: s
-    rule: HTHN.filter_acc.induct)
-  (cook mode = run_finish)
+  apply(induction "sat_is_un_1_list_fo1 y" _ _ arbitrary: s rule: HTHN.map_acc.induct)
+   apply(cook mode = run_finish)
+  done
 
-compile_nat HTHN.filter_prod_fsts_neq_nat_eq_unfolded
-HOL_To_IMP_correct HOL_To_HOL_Nat.filter_prod_fsts_neq_nat by cook
+compile_nat HTHN.sat_is_un_1_list_fo2_nat_eq_unfolded
+HOL_To_IMP_correct HOL_To_HOL_Nat.sat_is_un_1_list_fo2_nat
+  by cook
 
-lemmas map_filter_prod_fsts_neq_acc_nat_eq = HTHN.map_acc_filter_prod_fsts_neq_nat_eq_unfolded
-  [unfolded case_list_nat_def]
-compile_nat map_filter_prod_fsts_neq_acc_nat_eq
-HOL_To_IMP_correct HOL_To_HOL_Nat.map_acc_filter_prod_fsts_neq_nat
+lemmas map_acc_sat_is_un_1_list_fo2_nat_eq =
+  HTHN.map_acc_sat_is_un_1_list_fo2_nat_eq_unfolded[unfolded case_list_nat_def]
+compile_nat map_acc_sat_is_un_1_list_fo2_nat_eq
+HOL_To_IMP_correct HOL_To_HOL_Nat.map_acc_sat_is_un_1_list_fo2_nat
   apply (tactic \<open>HM.correct_if_IMP_tailcall_correct_tac HT.get_IMP_def @{context} 1\<close>)
-  by (induction "HTHN.filter_prod_fsts_neq :: (('a \<times> 'b) \<times> 'a \<times> 'c) list \<Rightarrow> _" _ _ arbitrary: s
-    rule: HTHN.map_acc.induct)
-  (cook mode = run_finish)
+  apply(induction "sat_is_un_1_list_fo2 :: ('a \<times> 'b list) \<Rightarrow> _" _ _ arbitrary: s rule: HTHN.map_acc.induct)
+   apply(cook mode = run_finish)
+  done
 
-end
-
-context HOL_To_HOL_Nat
-begin
-
-definition "pair_list \<equiv> \<lambda>(a, b). [a, b]"
-function_compile_nat pair_list_def
-
-definition "map_acc_pair_list \<equiv> map_acc pair_list"
-lemmas map_acc_pair_list_eq = map_acc_eq[of pair_list, folded map_acc_pair_list_def]
-function_compile_nat map_acc_pair_list_eq
-
-end
-
-context HOL_Nat_To_IMP
-begin
-
-lemmas pair_list_nat_eq = HTHN.pair_list_nat_eq_unfolded[unfolded case_prod_nat_def]
-compile_nat pair_list_nat_eq
-HOL_To_IMP_correct HOL_To_HOL_Nat.pair_list_nat by cook
-
-lemmas map_acc_pair_list_nat_eq = HTHN.map_acc_pair_list_nat_eq_unfolded[unfolded
-  case_list_nat_def]
-compile_nat map_acc_pair_list_nat_eq
-HOL_To_IMP_correct HOL_To_HOL_Nat.map_acc_pair_list_nat
-  apply (tactic \<open>HM.correct_if_IMP_tailcall_correct_tac HT.get_IMP_def @{context} 1\<close>)
-  by (induction "HTHN.pair_list :: ('a \<times> 'a) \<Rightarrow> _" _ _ arbitrary: s rule: HTHN.map_acc.induct)
-  (cook mode = run_finish)
-
-end
-
-context HOL_To_HOL_Nat
-begin
-
-definition "prod_product \<equiv> \<lambda>(a, b). List.product a b"
-function_compile_nat prod_product_def
-
-definition "map_acc_prod_product \<equiv> map_acc prod_product"
-lemmas map_acc_prod_product_eq = map_acc_eq[of prod_product, folded map_acc_prod_product_def]
-function_compile_nat map_acc_prod_product_eq
-
-end
-
-context HOL_Nat_To_IMP
-begin
-
-lemmas prod_product_nat_eq = HTHN.prod_product_nat_eq_unfolded[unfolded case_prod_nat_def]
-compile_nat prod_product_nat_eq
-HOL_To_IMP_correct HOL_To_HOL_Nat.prod_product_nat by (cook mode = induction)
-
-lemmas map_acc_prod_product_nat_eq = HTHN.map_acc_prod_product_nat_eq_unfolded[unfolded
-  case_list_nat_def]
-compile_nat map_acc_prod_product_nat_eq
-HOL_To_IMP_correct HOL_To_HOL_Nat.map_acc_prod_product_nat
-  apply (tactic \<open>HM.correct_if_IMP_tailcall_correct_tac HT.get_IMP_def @{context} 1\<close>)
-  by (induction "HTHN.prod_product :: 'a list \<times> 'b list \<Rightarrow> _" _ _ arbitrary: s
-    rule: HTHN.map_acc.induct)
-  (cook mode = run_finish)
+compile_nat HTHN.sat_is_un_1_list_nat_eq_unfolded
+HOL_To_IMP_correct HOL_To_HOL_Nat.sat_is_un_1_list_nat
+  by cook
 
 end
 
@@ -189,16 +99,49 @@ begin
 case_of_simps conflict_lit_eq : conflict_lit.simps
 function_compile_nat conflict_lit_eq
 
-definition "prod_fsts_conflict_lit \<equiv> \<lambda>((a, _), (b, _)). conflict_lit a b"
-lemma prod_fsts_conflict_lit_eq:
-  "prod_fsts_conflict_lit x = conflict_lit (fst (fst x)) (fst (snd x))"
-  unfolding prod_fsts_conflict_lit_def by auto
-function_compile_nat prod_fsts_conflict_lit_eq
+lemmas sat_is_un_2_list_fo0_eq = sat_is_un_2_list_fo0_def[unfolded case_prod_unfold]
+function_compile_nat sat_is_un_2_list_fo0_eq
 
-definition "filter_acc_prod_fsts_conflict_lit = filter_acc prod_fsts_conflict_lit"
-lemmas filter_acc_prod_fsts_conflict_lit_eq = filter_acc_eq[
-  of prod_fsts_conflict_lit, folded filter_acc_prod_fsts_conflict_lit_def]
-function_compile_nat filter_acc_prod_fsts_conflict_lit_eq
+definition "map_acc_sat_is_un_2_list_fo0 i_Ci j_Cj l1 \<equiv> map_acc (sat_is_un_2_list_fo0 i_Ci j_Cj l1)"
+lemmas map_acc_sat_is_un_2_list_fo0_eq =                 
+  map_acc_eq[of "sat_is_un_2_list_fo0 i_Ci j_Cj l1" for i_Ci j_Cj l1,
+    folded map_acc_sat_is_un_2_list_fo0_def]  
+function_compile_nat map_acc_sat_is_un_2_list_fo0_eq
+
+lemmas sat_is_un_2_list_fo1_eq =
+  sat_is_un_2_list_fo1_def[unfolded case_prod_unfold map_eq_map_acc_nil,
+    folded map_acc_sat_is_un_2_list_fo0_def]
+function_compile_nat sat_is_un_2_list_fo1_eq
+
+definition "map_acc_sat_is_un_2_list_fo1 i_Ci j_Cj \<equiv> map_acc (sat_is_un_2_list_fo1 i_Ci j_Cj)"
+lemmas map_acc_sat_is_un_2_list_fo1_eq =
+  map_acc_eq[of "sat_is_un_2_list_fo1 i_Ci j_Cj" for i_Ci j_Cj, folded map_acc_sat_is_un_2_list_fo1_def]
+function_compile_nat map_acc_sat_is_un_2_list_fo1_eq
+
+lemmas sat_is_un_2_list_fo2_eq =
+  sat_is_un_2_list_fo2_def[unfolded case_prod_unfold map_eq_map_acc_nil,
+    folded map_acc_sat_is_un_2_list_fo1_def]
+function_compile_nat sat_is_un_2_list_fo2_eq
+
+definition "map_acc_sat_is_un_2_list_fo2 i_Ci \<equiv> map_acc (sat_is_un_2_list_fo2 i_Ci)"
+lemmas map_acc_sat_is_un_2_list_fo2_eq =
+  map_acc_eq[of "sat_is_un_2_list_fo2 i_Ci" for i_Ci, folded map_acc_sat_is_un_2_list_fo2_def]
+function_compile_nat map_acc_sat_is_un_2_list_fo2_eq
+
+lemmas sat_is_un_2_list_fo3_eq =
+  sat_is_un_2_list_fo3_def[unfolded case_prod_unfold map_eq_map_acc_nil,
+    folded map_acc_sat_is_un_2_list_fo2_def]
+function_compile_nat sat_is_un_2_list_fo3_eq
+
+definition "map_acc_sat_is_un_2_list_fo3 F \<equiv> map_acc (sat_is_un_2_list_fo3 F)"
+lemmas map_acc_sat_is_un_2_list_fo3_eq =
+  map_acc_eq[of "sat_is_un_2_list_fo3 F" for F, folded map_acc_sat_is_un_2_list_fo3_def]
+function_compile_nat map_acc_sat_is_un_2_list_fo3_eq
+
+lemmas sat_is_un_2_list_fo_eq =
+  sat_is_un_2_list_fo_def[unfolded map_eq_map_acc_nil, folded map_acc_sat_is_un_2_list_fo3_def]
+function_compile_nat sat_is_un_2_list_fo_eq
+
 
 end
 
@@ -209,41 +152,68 @@ lemmas conflict_lit_nat_eq = HTHN.conflict_lit_nat_eq_unfolded[unfolded case_lit
 compile_nat conflict_lit_nat_eq
 HOL_To_IMP_correct HOL_To_HOL_Nat.conflict_lit_nat by cook
 
-lemmas prod_fsts_conflict_lit_nat_eq = HTHN.prod_fsts_conflict_lit_nat_eq_unfolded[unfolded case_prod_nat_def]
-compile_nat prod_fsts_conflict_lit_nat_eq
-HOL_To_IMP_correct HOL_To_HOL_Nat.prod_fsts_conflict_lit_nat by cook
+lemmas sat_is_un_2_list_fo0_nat_eq =
+  HTHN.sat_is_un_2_list_fo0_nat_eq_unfolded[unfolded case_prod_nat_def]
+compile_nat sat_is_un_2_list_fo0_nat_eq
+HOL_To_IMP_correct HOL_To_HOL_Nat.sat_is_un_2_list_fo0_nat
+  by cook
 
-lemmas filter_acc_prod_fsts_conflict_lit_nat_eq =
-  HTHN.filter_acc_prod_fsts_conflict_lit_nat_eq_unfolded[unfolded case_list_nat_def case_bool_nat_def]
-compile_nat filter_acc_prod_fsts_conflict_lit_nat_eq
-HOL_To_IMP_correct HOL_To_HOL_Nat.filter_acc_prod_fsts_conflict_lit_nat
+lemmas map_acc_sat_is_un_2_list_fo0_nat_eq =
+  HTHN.map_acc_sat_is_un_2_list_fo0_nat_eq_unfolded[unfolded case_list_nat_def]
+compile_nat map_acc_sat_is_un_2_list_fo0_nat_eq
+HOL_To_IMP_correct HOL_To_HOL_Nat.map_acc_sat_is_un_2_list_fo0_nat
   apply (tactic \<open>HM.correct_if_IMP_tailcall_correct_tac HT.get_IMP_def @{context} 1\<close>)
-  by (induction "HTHN.prod_fsts_conflict_lit :: ((('a lit \<times> 'b) \<times> ('a lit \<times> 'c)) \<Rightarrow> _) " _ _ arbitrary: s
-    rule: HTHN.filter_acc.induct)
-  (cook mode = run_finish)
+  apply(induction "sat_is_un_2_list_fo0 y ya yb" _ _ arbitrary: s rule: HTHN.map_acc.induct)
+   apply(cook mode = run_finish)
+  done
+
+compile_nat HTHN.sat_is_un_2_list_fo1_nat_eq_unfolded
+HOL_To_IMP_correct HOL_To_HOL_Nat.sat_is_un_2_list_fo1_nat
+  by cook
+
+lemmas map_acc_sat_is_un_2_list_fo1_nat_eq =
+  HTHN.map_acc_sat_is_un_2_list_fo1_nat_eq_unfolded[unfolded case_list_nat_def]
+compile_nat map_acc_sat_is_un_2_list_fo1_nat_eq
+HOL_To_IMP_correct HOL_To_HOL_Nat.map_acc_sat_is_un_2_list_fo1_nat
+  apply (tactic \<open>HM.correct_if_IMP_tailcall_correct_tac HT.get_IMP_def @{context} 1\<close>)
+  apply(induction "sat_is_un_2_list_fo1 y ya" _ _ arbitrary: s rule: HTHN.map_acc.induct)
+   apply(cook mode = run_finish)
+  done
+
+compile_nat HTHN.sat_is_un_2_list_fo2_nat_eq_unfolded
+HOL_To_IMP_correct HOL_To_HOL_Nat.sat_is_un_2_list_fo2_nat
+  by cook
+
+lemmas map_acc_sat_is_un_2_list_fo2_nat_eq =
+  HTHN.map_acc_sat_is_un_2_list_fo2_nat_eq_unfolded[unfolded case_list_nat_def]
+compile_nat map_acc_sat_is_un_2_list_fo2_nat_eq
+HOL_To_IMP_correct HOL_To_HOL_Nat.map_acc_sat_is_un_2_list_fo2_nat
+  apply (tactic \<open>HM.correct_if_IMP_tailcall_correct_tac HT.get_IMP_def @{context} 1\<close>)
+  apply(induction "sat_is_un_2_list_fo2 y" _ _ arbitrary: s rule: HTHN.map_acc.induct)
+   apply(cook mode = run_finish)
+  done
+
+compile_nat HTHN.sat_is_un_2_list_fo3_nat_eq_unfolded
+HOL_To_IMP_correct HOL_To_HOL_Nat.sat_is_un_2_list_fo3_nat
+  by cook
+
+lemmas map_acc_sat_is_un_2_list_fo3_nat_eq =
+  HTHN.map_acc_sat_is_un_2_list_fo3_nat_eq_unfolded[unfolded case_list_nat_def]
+compile_nat map_acc_sat_is_un_2_list_fo3_nat_eq
+HOL_To_IMP_correct HOL_To_HOL_Nat.map_acc_sat_is_un_2_list_fo3_nat
+  apply (tactic \<open>HM.correct_if_IMP_tailcall_correct_tac HT.get_IMP_def @{context} 1\<close>)
+  apply(induction "sat_is_un_2_list_fo3 y" _ _ arbitrary: s rule: HTHN.map_acc.induct)
+   apply(cook mode = run_finish)
+  done
+
+compile_nat HTHN.sat_is_un_2_list_nat_eq_unfolded
+HOL_To_IMP_correct HOL_To_HOL_Nat.sat_is_un_2_list_nat
+  by cook
 
 end
 
 context HOL_To_HOL_Nat
 begin
-
-lemmas sat_is_un_1_list_eq = sat_is_un_1_list_def[unfolded map_eq_map_acc_nil, folded
-  map_acc_case_prod_map_rpair_def[unfolded case_prod_map_rpair_def rpair_def
-    map_eq_map_acc_nil]
-  map_acc_product_def
-  map_acc_filter_prod_fsts_neq_def[unfolded filter_prod_fsts_neq_def prod_fsts_neq_def]
-  map_acc_pair_list_def[unfolded pair_list_def]]
-function_compile_nat sat_is_un_1_list_eq
-
-lemmas sat_is_un_2_list_eq = sat_is_un_2_list_def[unfolded map_eq_map_acc_nil
-  filter_eq_filter_acc_nil, folded
-  map_acc_case_prod_map_rpair_def[unfolded case_prod_map_rpair_def rpair_def
-    map_eq_map_acc_nil]
-  map_acc_prod_product_def[unfolded prod_product_def]
-  filter_acc_prod_fsts_conflict_lit_def[unfolded prod_fsts_conflict_lit_def]
-  map_acc_pair_list_def[unfolded pair_list_def]]
-
-function_compile_nat sat_is_un_2_list_eq
 
 lemmas sat_is_list_eq = sat_is_list_def[unfolded list_length_eq_length]
 function_compile_nat sat_is_list_eq
@@ -253,25 +223,20 @@ end
 context HOL_Nat_To_IMP
 begin
 
-compile_nat HTHN.sat_is_un_1_list_nat_eq_unfolded
-HOL_To_IMP_correct HOL_To_HOL_Nat.sat_is_un_1_list_nat by cook
-
-compile_nat HTHN.sat_is_un_2_list_nat_eq_unfolded
-HOL_To_IMP_correct HOL_To_HOL_Nat.sat_is_un_2_list_nat by cook
-
 compile_nat HTHN.sat_is_list_nat_eq_unfolded
 HOL_To_IMP_correct HOL_To_HOL_Nat.sat_is_list_nat by cook
 
 corollary sat_is_list_IMP_correct:
-  assumes "Rel_nat (s ''sat_is_list_nat.arg.x'') x"
+  assumes [transfer_rule]: "Rel_nat (s ''sat_is_list_nat.arg.x'') x"
   shows "terminates_with_res_IMP (tailcall_to_IMP sat_is_list_nat_IMP_tailcall) s
     ''sat_is_list_nat.ret'' (natify (sat_is_list x))"
 proof -
-  have "HTHN.sat_is_list_nat TYPE('a) (s ''sat_is_list_nat.arg.x'') = natify (sat_is_list x)"
-    using HTHN.sat_is_list_nat_eq_unfolded[OF assms]
-      HTHN.Rel_nat_sat_is_list_nat_unfolded[OF assms]
-    by (simp add: Rel_nat_iff_eq_natify)
-  then show ?thesis using sat_is_list_nat_IMP_correct[of s, OF assms] by simp
+  have "Rel_nat (HTHN.sat_is_list_nat TYPE('a) (s ''sat_is_list_nat.arg.x'')) (sat_is_list x)"
+    supply HTHN.sat_is_list_related_transfer[transfer_rule]
+    by transfer_prover
+  then show ?thesis
+    unfolding Rel_nat_iff_eq_natify
+    using sat_is_list_nat_IMP_correct[of s, OF assms] by simp
 qed
 
 end
